Lecture 2 code size

teaching/eutypes2018/code/state/Heap.fsti
@@ -5,10 +5,10 @@ module Heap
   val heap : Type
   val ref  : Type -> Type
 
-  val sel     : #a:Type -> heap -> ref a -> GTot a   (* in Ghost effect---meaning this *)
-  val addr_of : #a:Type -> ref a -> GTot nat         (* code can only be used in specs *)
+  val sel     : #a:Type -> heap -> ref a -> GTot a   (* in Ghost effect *)
+  val addr_of : #a:Type -> ref a -> GTot nat         (* in Ghost effect *)    
 
-  let modifies (s:set nat) (h0 h1 : heap) =
-    forall (a:Type) (r:ref a).{:pattern (sel h1 r)}
-        ~(addr_of r `mem` s) ==> sel h1 r == sel h0 r
+  let modifies (s:set nat) (h0 h1 : heap) 
+  
+  = forall a (r:ref a). ~(addr_of r `mem` s) ==> sel h1 r == sel h0 r
 // END: heap_model
