teaching/eutypes2018/code/state/CountST.fst
@@ -12,8 +12,7 @@ let rec count_st' (r:ref nat) (n:nat)
 
 let rec count_st (n:nat) 
   : ST nat (requires (fun _ -> True))
-           (ensures  (fun h0 x h1 -> x == n /\ 
-                                     modifies !{} h0 h1)) 
+           (ensures  (fun h0 x h1 -> x == n /\ modifies !{} h0 h1)) 
 = let r = alloc 0 in 
   count_st' r n; 
   !r
