teaching/eutypes2018/code/state/FibonacciST.fst
@@ -16,10 +16,10 @@ let rec fibonacci_st' (i:pos) (n:nat{n >= i}) (r1 r2:ref nat)
                                       sel h1 r2 = fibonacci n /\
                                       modifies !{r1,r2} h0 h1)) 
 = if i < n then
-    (let temp = !r2 in
-     r2 := !r1 + !r2;              (* fibonacci (i+1) = fibonacci i + fibonacci (i-1) *)
-     r1 := temp;                                       (* fibonacci i we already have *)
-     fibonacci_st' (i+1) n r1 r2)          (* tail-recursive call to compute the rest *)
+   (let temp = !r2 in
+    r2 := !r1 + !r2; (* fibonacci (i+1) = fibonacci i + fibonacci (i-1) *)
+    r1 := temp;                          (* fibonacci i we already have *)
+    fibonacci_st' (i+1) n r1 r2)  (* tail-recursion to compute the rest *)
 // END: fibonacci_stprime
 
 // BEGIN: fibonacci_st
