teaching/eutypes2018/code/state/ST.fsti
@@ -8,8 +8,9 @@ open FStar.ST
 // BEGIN: alloc
   val alloc : #a:Type -> init:a -> 
     ST (ref a) (requires (fun _ -> True))
-               (ensures  (fun h0 r h1 -> modifies !{} h0 h1 /\ sel h1 r == init /\
-                                         ~(h0 `contains` r) /\ h1 `contains` r))
+               (ensures  (fun h0 r h1 -> 
+                            modifies !{} h0 h1 /\ sel h1 r == init /\
+                            ~(h0 `contains` r) /\ h1 `contains` r))
 // END: alloc
 
 // BEGIN: ops
